fairness/comp_utils.v
@@ -202,17 +202,20 @@ Section OuterExposing.
       (* TODO: get rid of LMo and use appropriate fairness premise on mtr *)
       inner_obls_exposed lift_EAi state_rel lmtr (LMo := LMo) (AMi := ALMi).
   
-  Lemma outer_exposing_subtrace ltr tr i str
+  Lemma outer_exposing_subtrace_gen ltr tr i str
     lift_Gi lift_EAi state_rel
     (OUTER_CORR: outer_LM_trace_exposing lift_Gi lift_EAi state_rel ltr tr)
-    (SUB: subtrace tr i NOinfinity = Some str):
+    fin
+    (SUB: subtrace tr i fin = Some str)
+    len
+    (LEN: trace_len_is tr len)
+    (GE_LEN: NOmega.le len fin):    
     exists sltr, 
       outer_LM_trace_exposing lift_Gi lift_EAi state_rel sltr str.
   Proof. 
     red in OUTER_CORR. destruct OUTER_CORR as (UPTO & FAIR_AUX & INNER_OBLS).
-    pose proof (trace_has_len tr) as [len LEN].
-    pose proof SUB as X. eapply subtrace_equiv_after in X as (atr & AFTER & EQUIV); eauto.
-    2: { lia_NO len. }
+    pose proof SUB as X.
+    unshelve eapply subtrace_equiv_after in X as (atr & AFTER & EQUIV); eauto.  
     forward eapply upto_stutter_after; eauto. intros (i' & latr & AFTER' & UPTO').
     exists latr. split; [| split].
     - eauto. eapply upto_stutter_Proper; [.. |eapply UPTO']; eauto.
@@ -222,7 +225,44 @@ Section OuterExposing.
       forward eapply fair_by_gen_after; [apply AFTER' |..]; eauto.
       intros. apply FAIR_AUX.
     - eapply inner_obls_exposed_after; eauto.
-  Qed.   
+  Qed.
+
+  Lemma outer_exposing_subtrace ltr tr i str
+    lift_Gi lift_EAi state_rel
+    (OUTER_CORR: outer_LM_trace_exposing lift_Gi lift_EAi state_rel ltr tr)
+    (SUB: subtrace tr i NOinfinity = Some str):    
+    exists sltr, 
+      outer_LM_trace_exposing lift_Gi lift_EAi state_rel sltr str.
+  Proof.
+    pose proof (trace_has_len tr) as [len LEN].
+    eapply outer_exposing_subtrace_gen; eauto.
+    lia_NO len. 
+  Qed.
+  
+  Lemma outer_exposing_after ltr tr i atr
+    lift_Gi lift_EAi state_rel
+    (OUTER_CORR: outer_LM_trace_exposing lift_Gi lift_EAi state_rel ltr tr)
+    (AFTER: after i tr = Some atr):
+    exists sltr, 
+      outer_LM_trace_exposing lift_Gi lift_EAi state_rel sltr atr.
+  Proof.
+    pose proof (trace_has_len tr) as [len LEN].
+    forward eapply subtrace_len with (start := i); eauto. 
+    2: reflexivity.
+    { apply state_lookup_after_0 in AFTER.
+      eapply mk_is_Some, state_lookup_dom in AFTER; eauto. }
+
+    intros (str & SUB & LENs).
+    pose proof SUB as SUB_. 
+    eapply subtrace_equiv_after in SUB; eauto.
+    2: reflexivity.
+    destruct SUB as (atr_ & AFTER_ & EQ).
+    rewrite AFTER_ in AFTER. inversion AFTER. subst.
+
+    apply traces_equiv_eq in EQ as ->.
+    eapply outer_exposing_subtrace_gen; eauto.
+    reflexivity. 
+  Qed.
   
 End OuterExposing.
 
